
Bijzondere gevallen:
- $\sin(x)=-1 =>x=1\frac{1}{2}\pi+k.2\pi$
- $\sin(x)=0 =>x=0+k.\pi$
- $\sin(x)=1 =>x=\frac{1}{2}\pi+k.2\pi$
- $\cos(x)=-1 =>x=\pi+k.2\pi$
-  $\cos(x)=0 =>x=\frac{1}{2}\pi+k.\pi$
- $\cos(x)=1 =>x=0+k.2\pi$
- $\tan(x)=0=>x=k.\pi$

Vergelijkingen
- $\sin(x)=\alpha=>x=\alpha+k.2\pi\lor x=\pi-\alpha+k.2\pi$
- $\cos(x)=\alpha=>x=\alpha+k.2\pi\lor x=-\alpha+k.2\pi$
- $\tan(x)=\alpha=>x=\alpha+k.\pi$

Regels
- $\sin(2x)=2\sin(x)\cos(x)$
- $\begin{align} \cos(2x)=\cos^{2}(x)-\sin^{2}(x)\\ =2\cos^{2}(x)-1\\ =1-\sin^{2}(x)\end{align}$



Formules
- $\sin^{2}(x)=\frac{1}{2}-\frac{1}{2}\cos(2x)$
- $\cos^{2}(x)=\frac{1}{2}+\frac{1}{2}\cos(2x)$
- $a\cos(2x)+b\sin(2x)+c$
- $\tan\alpha=\frac{b}{a}$
- $\sqrt{a^{2}+b^{2}}\cos(2x-\alpha)+c$

$$\dfrac{-2\sqrt{3}\sin^{2}(x)+\sin(2x)}{3^{2x}-8.3^{x}-9} \ge 0 \quad x \in \mathbb{}[-\pi,\pi]$$

$$
\begin{align}
T=0 =>-2\sqrt{3}\sin^{2}(x)+\sin(2x)=0\\[8pt]
-2\sqrt{3}(\frac{1}{2}-\frac{1}{2}\cos(2x))+\sin(2x)=0\\ [8pt]
-\sqrt{3}+\sqrt{3}\cos(2x)+\sin(2x)=0\\[8pt]
\sqrt{3}\cos(2x)+\sin(2x)-\sqrt{3}=0
\end{align}
$$
$$
\begin{align}
a\cos(2x)+b\sin(2x)+c\\
\tan(\phi)=\frac{b}a{}
\end{align}
$$
![[Group 41.png]]
$$
\begin{align}
\tan(\phi)=\frac{1}{\sqrt{3}} \quad eerste \ kw\\
\phi=\frac{1}{6}\pi\\
\sqrt{(\sqrt{3})^{2}+(1)^{2}}\cos(2x-\frac{1}{6}\pi)-\sqrt{3}=0\\
2\cos(2x-\frac{1}{6}\pi)-\sqrt{3}=0\\
\cos(2x-\frac{1}{6}\pi)=\frac{1}{2}\sqrt{3}\\
2x-\frac{1}{6}\pi=\frac{1}{6}\pi+k.2\pi\ \lor 2x-\frac{1}{6}\pi=-\frac{1}{6}\pi+k.2\pi\\
x=\frac{1}{6}\pi+k.\pi \ \lor x=k.\pi\\
\{-\pi,-\frac{5}{6}\pi,0,\frac{1}{6}\pi,\pi \}
\end{align}
$$
$$ 
\begin{align}
N=0=>3^{2x}-8.3{x}-9=0\\
Stel:3^{x}=u\\
u^{2}-8u-9=0\\
(u-9)(u+1)=0\\
u=9\lor u=-1\\
3^{x}=9\lor 3^{x}=-1\\
x=2\lor \emptyset
\end{align}
$$
![[Group 42.png]]
![[Group 50.png]]


$$[-\pi,-\frac{5}{6}\pi]\lor[0,2\rangle\lor\{\pi\}$$

$$\dfrac{3^{x+2}+3^{x-1}-84}{-2\sqrt{3}sin^{2}(x)-2\sin(x)cos(x)+2\sqrt{3}} \le 0 \ \ x \in \mathbb{}  [\pi,\pi] $$

$$
\begin{align}
T=0=>3^{x+2}+3^{x-1}-84=0\\
3^{x+2}+3^{x-1}-3^{5}=0\\
x+2+x-1-5=0\\
2x-4=0\\
x=2
\end{align}
$$

![[Group 43.png]]
$$
\begin{align}
N=0 =>-2\sqrt{3}sin^{2}(x)-2\sin(x)cos(x)+2\sqrt{3}=0\\
-2\sqrt{3}(\frac{1}{2}-\frac{1}{2}\cos(2x))-\sin(2x)+2\sqrt{3}=0\\
-\sqrt{3}+\sqrt{3}\cos(2x)-sin(2x)+2\sqrt{3}=0\\
\sqrt{3}\cos(2x)-\sin(2x)+\sqrt{3}=0\\
\end{align}
$$
$$
\begin{align}
a=\sqrt{3} \ \land b=-1 \land \ c=\sqrt{3} \\
\tan\phi=\frac{-1}{\sqrt{3}}\ 4e\ kw\\
\phi=1\frac{5}{6}\pi
\end{align}
$$
$$\begin{align}
\sqrt{(\sqrt{3})^{2}+(-1)^{2}}\cos(2x-1\frac{5}{6}\pi)+\sqrt{3}=0\\
2\cos(2x-1\frac{5}{6}\pi)=-\sqrt{3}\\
2x-1\frac{5}{6}\pi=\frac{5}{6}\pi+k.2\pi \ \lor 2x-1\frac{5}{6}\pi=-\frac{5}{6}\pi+k.2\pi\\
x=1\frac{1}{3}\pi+k.\pi \ \lor x=\frac{1}{2}\pi+k.\pi\\
\{-\frac{1}{2}\pi,-\frac{1}{3}\pi,\frac{1}{2}\pi\}
\end{align}
$$

![[Group 51.png]]
$$[-\pi,2] \backslash \{-\frac{1}{2}\pi,\frac{1}{3}\pi,\frac{1}{2}\pi\}\lor \{\pi\}$$

$$\dfrac{1-\cos^{2}(x)+\sin^{2}(x)+2\sin(x)\cos(x)}{2^{x}-9.2^{x+1}+32} \le0\quad x \in \mathbb{}[0,\pi] $$
$$
\begin{align}
1-(\frac{1}{2}+\frac{1}{2}\cos(2x))+(\frac{1}{2}-\frac{1}{2}\cos(2x))+\sin(2x)=0\\
-\cos(2x)+\sin(2x)+1=0\\
a=-1\land b=1\land c=1
\end{align}
$$
$$
\begin{align}
\tan\phi=\frac{1}{-1} ->2e\ kw\\
\phi=\frac{3}{4}\pi
\end{align}
$$

$$
\begin{align}
T=0=>
\sqrt{(-1)^{2}+(1)^{2}}\cos(2x-\frac{3}{4}\pi)+1=0\\
\sqrt{2}\cos(2x-\frac{3}{4}\pi)+1=0\\
\cos(2x-\frac{3}{4}\pi)=-\frac{1}{2}\sqrt{2}\\
2x-\frac{3}{4}\pi=\frac{3}{4}\pi+k.2\pi\ \lor 2x-\frac{3}{4}\pi=-\frac{3}{4}\pi+k.2\pi\\
x=\frac{3}{4}\pi+k.\pi \ \lor x=k.\pi\\
\{0,\frac{3}{4}\pi,\pi\}
\end{align}
$$

$$
\begin{align}
stel:\ 2^{x}=u\\
u^{2}-18u+32=0\\
(u-16)(u-2)=0\\
u=16\ \lor u=2\\
x=4 \ VN\ \lor x=1
\end{align}
$$
![[Group 52.png]]



![[Group 56.png]]

$$\{0,\pi\}\lor \langle1,\frac{3}{4}\pi]$$

$$\dfrac{2\sin^{2}(x)+\sqrt{3}\sin(2x)+1}{e^{2x}-2e^{x}-3}\ge 0 \quad x \in \mathbb{}[-\pi,\pi] $$
$$
\begin{align}
T=0 =>2\sin^{2}(x)+\sqrt{3}\sin(2x)+1=0\\
2(\frac{1}{2}-\frac{1}{2}\cos(2x))+\sqrt{3}\sin(2x)+1=0\\
1-\cos(2x)+\sqrt{3}\sin(2x)+1=0\\
-\cos(2x)+\sqrt{3}\sin(2x)+2=0\\
a=-1\land b=\sqrt{3}\land c=2
\end{align}
$$

$$
\begin{align}
\tan\phi=\frac{\sqrt{3}}{-1}=> 2e\ kw\\
\phi=\frac{2}{3}\pi
\end{align}
$$
$$
\begin{align}
\sqrt{(-1)^{2}+(\sqrt{3})^{2}}\cos(2x-\frac{2}{3}\pi)+2=0\\
2\cos(2x-\frac{2}{3}\pi)+2=0\\
\cos(2x-\frac{2}{3}\pi)=-1\\
2x-\frac{2}{3}\pi=\pi+k.2\pi\\
x=\frac{5}{6}\pi+k.\pi\\
\{-\frac{1}{6}\pi,\frac{5}{6}\pi\}
\end{align}
$$
$$
\begin{align}
N=0=>e^{2x}-2e^{x}-3=0\\
(e^{x}-3)(e^{x}+1)=0\\
e^{x}=3\lor e^{x}=-1\\
x=\ln(3) \lor \emptyset
\end{align}
$$
![[Group 59.png]]

![[Group 63.png]]

$$[-\pi,\ln(3)\rangle\lor\{\frac{5}{6}\pi,\pi\}$$